theories/ftlr/ftlr_base.v
@@ -10,7 +10,7 @@ Section fundamental.
     {ceriseg:ceriseG Σ} {sealsg: sealStoreG Σ}
     {Cname : CmptNameG}
     {stsg : STSG Addr region_type Σ} {heapg : heapGS Σ}
-    {tframeg : TFRAMEG Σ}
+    {cstackg : CSTACKG Σ}
     {nainv: logrel_na_invs Σ}
     `{MP: MachineParameters}
     {swlayout : switcherLayout}
@@ -20,7 +20,7 @@ Section fundamental.
   Notation STS_STD := (leibnizO (STS_std_states Addr region_type)).
   (* Notation TFRAME := (leibnizO nat). *)
   Notation WORLD := (prodO STS_STD STS).
-  Notation STK := (leibnizO (list (Word * Word))).
+  Notation CSTK := (leibnizO cstack).
   Implicit Types W : WORLD.
   Implicit Types C : CmptName.
 
@@ -33,22 +33,22 @@ Section fundamental.
     executeAllowed p = true ∧ (isWL p = true -> g = Local).
 
   Definition ftlr_IH: iProp Σ :=
-    (□ ▷ (∀ (W_ih : WORLD) (C_ih : CmptName) (stk : STK) (r_ih : leibnizO Reg)
-            (p_ih : Perm) (g_ih : Locality) (b_ih e_ih a_ih : Addr) (cstk_ih : Word),
+    (□ ▷ (∀ (W_ih : WORLD) (C_ih : CmptName) (cstk : CSTK) (r_ih : leibnizO Reg)
+            (p_ih : Perm) (g_ih : Locality) (b_ih e_ih a_ih : Addr) (wstk_ih : Word),
             full_map r_ih
             -∗ (∀ (r : RegName) v, ⌜r ≠ PC⌝ → ⌜r_ih !! r = Some v⌝ → interp W_ih C_ih v)
-            -∗ registers_pointsto (<[PC:= WCap p_ih g_ih b_ih e_ih a_ih]> (<[csp:=cstk_ih]> r_ih))
+            -∗ registers_pointsto (<[PC:= WCap p_ih g_ih b_ih e_ih a_ih]> (<[csp:=wstk_ih]> r_ih))
             -∗ region W_ih C_ih
             -∗ sts_full_world W_ih C_ih
-            -∗ interp_continuation stk W_ih C_ih
+            -∗ interp_continuation cstk W_ih C_ih
             -∗ na_own logrel_nais ⊤
-            -∗ tframe_frag stk
+            -∗ cstack_frag cstk
             -∗ □ interp W_ih C_ih (WCap p_ih g_ih b_ih e_ih a_ih)
             -∗ interp_conf W_ih C_ih))%I.
 
   Definition ftlr_instr_base (W : WORLD) (C : CmptName) (regs : leibnizO Reg)
     (p p' : Perm) (g : Locality) (b e a : Addr)
-    (w : Word) (ρ : region_type) (P : D) (Pinstr : Prop) (stk : STK) (cstk : Word)
+    (w : Word) (ρ : region_type) (P : D) (Pinstr : Prop) (cstk : CSTK) (wstk : Word)
     (Nswitcher : namespace)
     : Prop :=
     validPCperm p g
@@ -79,15 +79,15 @@ Section fundamental.
                  else (if isDL p' then future_borrow_mono C (safeC P) w else future_priv_mono C (safeC P) w))
            else future_priv_mono C (safeC P) w))
     -∗ ▷ P W C w
-    -∗ interp_continuation stk W C
+    -∗ interp_continuation cstk W C
     -∗ sts_full_world W C
     -∗ na_own logrel_nais ⊤
-    -∗ tframe_frag stk
+    -∗ cstack_frag cstk
     -∗ open_region W C a
     -∗ sts_state_std C a ρ
     -∗ a ↦ₐ w
     -∗ PC ↦ᵣ (WCap p g b e a)
-    -∗ ([∗ map] k↦y ∈ delete PC (<[csp:=cstk]> regs), k ↦ᵣ y)
+    -∗ ([∗ map] k↦y ∈ delete PC (<[csp:=wstk]> regs), k ↦ᵣ y)
     -∗ na_inv logrel_nais Nswitcher switcher_inv (** SWITCHER INVARIANT *)
     -∗ WP Instr Executable
         {{ v, WP Seq (cap_lang.of_val v)
@@ -96,9 +96,9 @@ Section fundamental.
 
   Definition ftlr_instr (W : WORLD) (C : CmptName) (regs : leibnizO Reg)
     (p p' : Perm) (g : Locality) (b e a : Addr)
-    (w : Word) (i: instr) (ρ : region_type) (P : D) (stk : STK) (cstk : Word)
+    (w : Word) (i: instr) (ρ : region_type) (P : D) (cstk : CSTK) (wstk : Word)
     (Nswitcher : namespace)
     : Prop :=
-    ftlr_instr_base W C regs p p' g b e a w ρ P (decodeInstrW w = i) stk cstk Nswitcher.
+    ftlr_instr_base W C regs p p' g b e a w ρ P (decodeInstrW w = i) cstk wstk Nswitcher.
 
 End fundamental.
